Vars.v
@@ -1,0 +1,199 @@
+(** Calculation of the simple arithmetic language. *)
+
+Require Import Tactics.
+Require Export Memory.
+Module Arith (mem : MemoryExt).
+Import mem.
+
+(** * Syntax *)
+
+Inductive var := X | Y | Z.
+
+Inductive Expr : Set :=
+| Val : nat -> Expr 
+| Add : Expr -> Expr -> Expr
+| Var : var -> Expr.
+
+(** * Semantics *)
+
+Definition env := var -> nat.
+
+Fixpoint eval (e : env) (x: Expr) : nat :=
+  match x with
+    | Val n => n
+    | Add x1 x2 => eval e x1 + eval e x2
+    | Var v => e v
+  end.
+
+(** * Compiler *)
+
+Inductive Code : Set :=
+| LOAD : nat -> Code -> Code
+| LDA : adr -> Code -> Code
+| ADD : adr -> Code -> Code
+| STORE : adr -> Code -> Code
+| HALT : Code.
+
+Fixpoint comp' (x : Expr) (vars: var -> adr) (r : adr) (c : Code) : Code :=
+  match x with
+  | Val n => LOAD n c
+  | Add x1 x2 => comp' x1  vars r (STORE r (comp' x2 vars (next r) (ADD r c)))
+  | Var v => LDA (vars v) c
+  end.
+
+Definition mkVars : var -> adr :=
+  fun v =>
+    match v with
+    | X => first
+    | Y => next first
+    | Z => next (next first)
+    end.
+
+Definition firstFresh : adr := next (next (next first)).
+
+Definition mkMem (e : env) : Mem :=
+  set (mkVars Z) (e Z) ((set (mkVars Y) (e Y) (set (mkVars X) (e X) empty))).  
+  
+  
+Definition comp (x : Expr) : Code := comp' x mkVars firstFresh HALT.
+
+(** * Virtual Machine *)
+
+Definition Memory : Type := Mem.
+Definition Acc : Type := nat.
+
+Definition Conf : Type := (Code * Memory * Acc)%type.
+
+Reserved Notation "x ==> y" (at level 80, no associativity).
+Inductive VM : Conf -> Conf -> Prop :=
+| vm_load n c m a : (LOAD n c , m, a) ==> (c , m, n)
+| vm_add c r m a : (ADD r c, m, a) ==> (c, free r m, get r m + a)
+| vm_store c r m a : (STORE r c, m, a) ==> (c, set r a m, a)
+| vm_lda c r m a : (LDA r c, m, a) ==> (c, m, get r m)
+where "x ==> y" := (VM x y).
+
+(** * Calculation *)
+
+(** Boilerplate to import calculation tactics *)
+
+Module VM <: Preorder.
+Definition Conf := Conf.
+Definition VM := VM.
+End VM.
+Module VMCalc := Calculation VM.
+Import VMCalc.
+
+Lemma env_fresh (e : env) vars r m
+  (Fresh : forall v, vars v < r)
+  (Env : forall v, e v = get (vars v) m) v n:
+  e v = get (vars v) (set r n m).
+Proof.
+  rewrite get_set'; auto using next_fresh.
+Qed.
+  
+  
+(** Specification of the compiler *)
+
+Theorem spec x r c a m vars e
+  (Fresh : forall v, vars v < r)
+  (Env : forall v, e v = get (vars v) m):
+  freeFrom r m ->
+  (comp' x vars r c, m, a) =>> (c , m, eval e x).
+
+(** Setup the induction proof *)
+
+Proof.
+  intros.
+  generalize dependent c.
+  generalize dependent m.
+  generalize dependent r.
+  generalize dependent a.
+  induction x;intros.
+
+(** Calculation of the compiler *)
+
+(** - [x = Val n]: *)
+
+  begin
+  (c, m, n).
+  <== { apply vm_load }
+  (LOAD n c, m, a).
+  [].
+
+(** - [x = Add x1 x2]: *)
+
+  begin
+    (c, m, eval e x1 + eval e x2).
+  = {rewrite freeFrom_free, get_set}
+    (c, free r (set r (eval e x1) m), get r (set r (eval e x1) m)  + eval e x2).
+  <== {apply vm_add}
+    (ADD r c, set r (eval e x1) m, eval e x2).
+  <<= {apply IHx2; auto using freeFrom_set, env_fresh}
+    (comp' x2 vars (next r) (ADD r c), set r (eval e x1) m, eval e x1).
+  <== {apply vm_store}
+    (STORE r (comp' x2 vars (next r) (ADD r c)), m, eval e x1).
+  <<= { apply IHx1}
+    (comp' x1 vars r (STORE r (comp' x2 vars (next r) (ADD r c))), m, a).
+  [].
+
+(** - [x = Var v]: *)
+  
+  begin
+    (c, m, e v).
+  = {rewrite Env}
+    (c, m, get (vars v) m).
+  <<= {apply vm_lda}
+    (LDA (vars v) c , m, a).  
+  [].
+Qed.
+
+
+Lemma mkMemEnv (e : env) (v : var) : e v = get (mkVars v) (mkMem e).
+Proof.
+  destruct v;
+  unfold mkMem; simpl;
+    repeat first [rewrite get_set' by (apply next_fresh; auto) | rewrite get_set];
+    reflexivity.
+Qed.
+
+Lemma mkVarsFresh v : mkVars v < firstFresh.
+Proof.
+  unfold firstFresh. destruct v; simpl; auto.
+Qed.
+
+Lemma freeFromFirst e : freeFrom firstFresh (mkMem e).
+Proof.
+  unfold mkMem. simpl. eauto using freeFrom_first, freeFrom_set.
+Qed. 
+
+Theorem spec_top x a e:
+  (comp x, mkMem e, a) =>> (HALT , mkMem e, eval e x).
+Proof.
+  apply spec.
+  - apply mkVarsFresh.
+  - apply mkMemEnv.
+  - apply freeFromFirst.
+Qed. 
+
+
+(** * Soundness *)
+  
+(** Since the VM is defined as a small step operational semantics, we
+have to prove that the VM is deterministic and does not get stuck in
+order to derive soundness from the above theorem. *)
+
+
+Lemma determ_vm : determ VM.
+  intros C C1 C2 V. induction V; intro V'; inversion V'; subst; reflexivity.
+Qed.
+
+
+Theorem sound x a C e : (comp x, mkMem e, a) =>>! C -> C = (HALT , mkMem e, eval e x).
+Proof.
+  intros.
+  pose (spec_top x) as H'. unfold comp in *. pose (determ_trc determ_vm) as D.
+  unfold determ in D. eapply D. apply H. split. apply H'. intro Contra. destruct Contra.
+  inversion H0.
+Qed.
+
+End Arith.
