Makefile
@@ -53,13 +53,16 @@ COQLIBS?=\
   -R "." ""\
   -R "." ""\
   -R "." ""\
+  -R "." ""\
   -R "." ""
 COQCHKLIBS?=\
   -R "." ""\
   -R "." ""\
   -R "." ""\
+  -R "." ""\
   -R "." ""
 COQDOCLIBS?=\
+  -R "." ""\
   -R "." ""\
   -R "." ""\
   -R "." ""\
@@ -108,7 +111,8 @@ endif
 VFILES:=Memory.v\
   LinearMemory.v\
   Tactics.v\
-  Arith.v
+  Arith.v\
+  Vars.v
 
 ifneq ($(filter-out archclean clean cleanall printenv,$(MAKECMDGOALS)),)
 -include $(addsuffix .d,$(VFILES))
